ID_system_formalisation/Centralised_Model.thy
@@ -1,0 +1,208 @@
+theory Centralised_Model imports
+  CryptHOL.CryptHOL
+begin
+
+sledgehammer_params[timeout = 1000]
+
+type_synonym ('user', 'result') query = "'user' \<Rightarrow> 'result'"
+
+type_synonym ('store_sens_attrs') govt_store_data = "'store_sens_attrs' set"
+
+locale centralised_id = 
+  fixes reg :: "'user \<Rightarrow> ('token \<times> ('store_sens_attrs) govt_store_data) spmf"
+    and auth :: "'token \<Rightarrow> ('user, 'query_out) query  \<Rightarrow> 'auth_token spmf"
+    and ver :: "'auth_token \<Rightarrow> 'query_out spmf"
+    and valid_user :: "'user \<Rightarrow> bool"
+    and valid_query :: "('user, 'query_out) query \<Rightarrow> bool"
+  assumes lossless_reg_user: "lossless_spmf (reg user)"
+begin
+    
+definition correct_game :: "'user \<Rightarrow> ('user, 'query_out) query  \<Rightarrow> bool spmf"
+  where 
+    "correct_game user query = do {
+      (token, govt_output) \<leftarrow> reg user;
+      auth_token \<leftarrow> auth token query;
+      result \<leftarrow> ver auth_token;
+      return_spmf (result = query user)}"
+
+definition "correct \<longleftrightarrow> (\<forall> user query. valid_user user \<longrightarrow> valid_query query 
+                            \<longrightarrow> spmf (correct_game user query) True = 1)"
+
+primrec sens_attrs_hiding_game :: "((('user \<times> 'user) \<times> 'state) spmf \<times> ('state \<Rightarrow> 'store_sens_attrs set \<Rightarrow> bool spmf)) \<Rightarrow> bool spmf"
+  where 
+    "sens_attrs_hiding_game (\<A>1, \<A>2) = TRY do { 
+      ((user0, user1), \<sigma>) \<leftarrow> \<A>1;
+      _ :: unit \<leftarrow> assert_spmf (valid_user user0 \<and> valid_user user1);      
+      b \<leftarrow> coin_spmf;
+      (card, (sens_attrs)) \<leftarrow> reg (if b then user0 else user1);
+      b' \<leftarrow> \<A>2 \<sigma> sens_attrs;
+      return_spmf (b' = b)} ELSE coin_spmf"
+
+definition "sens_attrs_hiding_advantage \<A> = \<bar>spmf (sens_attrs_hiding_game \<A>) True - 1/2\<bar>"
+
+definition "perfect_sens_attrs_hiding \<A> \<longleftrightarrow> sens_attrs_hiding_advantage \<A> = 0"
+
+lemma no_sens_attrs_imp_perfect_sens_attrs_hiding:
+  assumes "\<forall> user token store_non_sens_attr store_sens_attr. (token, store_sens_attr) \<in> set_spmf (reg user) \<longrightarrow> store_sens_attr = {}"
+  shows "perfect_sens_attrs_hiding \<A>"
+proof-
+  note [simp] = Let_def split_def 
+  have "\<bar>spmf (sens_attrs_hiding_game \<A>) True - 1/2\<bar> = 0"
+  proof-
+    obtain \<A>1 and \<A>2 where \<A> [simp]: "\<A> = (\<A>1, \<A>2)" by(cases \<A>)
+    have "sens_attrs_hiding_game (\<A>1, \<A>2) = TRY do {
+      ((user0, user1), \<sigma>) \<leftarrow> \<A>1;
+      _ :: unit \<leftarrow> assert_spmf (valid_user user0 \<and> valid_user user1);
+      b :: bool \<leftarrow> coin_spmf;
+      (card, (store_sens_attrs)) \<leftarrow> reg (if b then user0 else user1);
+      b' \<leftarrow> \<A>2 \<sigma> store_sens_attrs;
+      return_spmf (b' = b)} ELSE coin_spmf"
+      by(simp add: sens_attrs_hiding_game_def)
+    also have "... = TRY do {
+      ((user0, user1), \<sigma>) \<leftarrow> \<A>1;
+      _ :: unit \<leftarrow> assert_spmf (valid_user user0 \<and> valid_user user1);
+      b :: bool \<leftarrow> coin_spmf;
+      (card, (store_sens_attrs)) \<leftarrow> reg (if b then user0 else user1);
+      b' \<leftarrow> \<A>2 \<sigma> {};
+      return_spmf (b' = b)} ELSE coin_spmf"
+      apply auto
+      apply(intro try_spmf_cong bind_spmf_cong[OF refl]; clarsimp?)+
+      apply(intro bind_spmf_cong bind_spmf_cong[OF refl]; clarsimp?)
+      using assms by auto
+    also have "... = TRY do {
+      ((user0, user1), \<sigma>) \<leftarrow> \<A>1;
+      _ :: unit \<leftarrow> assert_spmf (valid_user user0 \<and> valid_user user1);
+      b' \<leftarrow> \<A>2 \<sigma> {};
+      map_spmf((=) b') coin_spmf} ELSE coin_spmf"
+      including monad_normalisation
+      apply(simp add: bind_spmf_const lossless_reg_user lossless_weight_spmfD) 
+      by(simp add: map_spmf_conv_bind_spmf)
+    also have "... = coin_spmf" 
+      by(auto simp add: bind_spmf_const map_eq_const_coin_spmf try_bind_spmf_lossless2' scale_bind_spmf weight_spmf_le_1 scale_scale_spmf)
+    ultimately show ?thesis  
+      by(simp add: spmf_of_set)
+  qed
+  thus ?thesis 
+    by(simp add: perfect_sens_attrs_hiding_def sens_attrs_hiding_advantage_def)
+qed
+
+
+
+
+end 
+
+end
+
+
+
+
+
+(*locale centralised_id = 
+  fixes user_enc_reg_phase :: "'sens_atrrs set \<Rightarrow> 'enc_sens_atrrs set spmf"
+  fixes govt_reg_phase :: "'attrs set \<Rightarrow> 'enc_sens_atrrs set \<Rightarrow> ('token \<times> ('store_non_sens_attrs, 'store_sens_attrs) govt_store_data) spmf"
+    and auth :: "'token \<Rightarrow> ('user, 'query_out) query  \<Rightarrow> 'auth_token spmf"
+    and ver :: "'auth_token \<Rightarrow> 'query_out spmf"
+    and valid_user :: "'user \<Rightarrow> bool"
+    and valid_query :: "('user, 'query_out) query \<Rightarrow> bool"
+    and users_attr_creation :: "'user \<Rightarrow> ('attrs set \<times> 'sens_atrrs set)"
+begin
+
+definition reg :: "'user \<Rightarrow> ('token \<times> ('store_non_sens_attrs, 'store_sens_attrs) govt_store_data) spmf"
+  where "reg user = do {
+    let (non_sens_attrs, sens_attrs) = users_attr_creation user;
+    enc_sens_attr \<leftarrow> user_enc_reg_phase sens_attrs;
+    
+definition correct_game :: "'user \<Rightarrow> ('user, 'query_out) query  \<Rightarrow> bool spmf"
+  where 
+    "correct_game user query = do {
+      (token, govt_output) \<leftarrow> reg user;
+      auth_token \<leftarrow> auth token query;
+      result \<leftarrow> ver auth_token;
+      return_spmf (result = query user)}"
+
+definition "correct \<longleftrightarrow> (\<forall> user query. valid_user user \<longrightarrow> valid_query query 
+                            \<longrightarrow> spmf (correct_game user query) True = 1)"
+
+primrec sens_attrs_hiding_game :: "((('user \<times> 'user) \<times> 'state) spmf \<times> ('state \<Rightarrow> 'store_sens_attrs set \<Rightarrow> bool spmf)) \<Rightarrow> bool spmf"
+  where 
+    "sens_attrs_hiding_game (\<A>1, \<A>2) = TRY do { 
+      ((user0, user1), \<sigma>) \<leftarrow> \<A>1;
+      _ :: unit \<leftarrow> assert_spmf (valid_user user0 \<and> valid_user user1);      
+      b \<leftarrow> coin_spmf;
+      (card, (non_sens_attrs, sens_attrs)) \<leftarrow> reg (if b then user0 else user1);
+      b' \<leftarrow> \<A>2 \<sigma> sens_attrs;
+      return_spmf (b' = b)} ELSE coin_spmf"
+
+definition "sens_attrs_hiding_advantage \<A> = \<bar>spmf (sens_attrs_hiding_game \<A>) True - 1/2\<bar>"
+
+definition "perfect_sens_attrs_hiding \<A> \<longleftrightarrow> sens_attrs_hiding_advantage \<A> = 0"
+
+definition "no_sens_attr \<longleftrightarrow> (\<forall> user. snd (users_attr_creation user) = {})"
+
+lemma 
+  assumes "no_sens_attr"
+  shows "perfect_sens_attrs_hiding' \<A>"
+  including monad_normalisation
+proof-
+  note [simp] = Let_def split_def 
+  have "\<bar>spmf (sens_attrs_hiding_game' \<A>) True - 1/2\<bar> = 0"
+  proof-
+    obtain \<A>1 and \<A>2 where \<A> [simp]: "\<A> = (\<A>1, \<A>2)" by(cases \<A>)
+    have "sens_attrs_hiding_game' (\<A>1, \<A>2) = TRY do {
+      ((user0, user1), \<sigma>) \<leftarrow> \<A>1;
+      _ :: unit \<leftarrow> assert_spmf (valid_user user0 \<and> valid_user user1);
+      b :: bool \<leftarrow> coin_spmf;
+      let (attrs, sens_attrs) = users_attr_creation (if b then user0 else user1);
+      enc_attrs \<leftarrow> reg_enc_sens_attrs sens_attrs;
+      (S, \<sigma>') \<leftarrow> reg_govt_shares attrs enc_attrs;
+      b' \<leftarrow> \<A>2 \<sigma> S;
+      return_spmf (b' = b)} ELSE coin_spmf"
+      by(simp add: sens_attrs_hiding_game_def reg_def bind_spmf_const lossless_reg_govt_token lossless_weight_spmfD)
+    also have "... = TRY do {
+      ((user0, user1), \<sigma>) \<leftarrow> \<A>1;
+      _ :: unit \<leftarrow> assert_spmf (valid_user user0 \<and> valid_user user1);
+      b :: bool \<leftarrow> coin_spmf;
+      let (attrs, sens_attrs) = users_attr_creation (if b then user0 else user1);
+      enc_attrs \<leftarrow> reg_enc_sens_attrs {};
+      (S, \<sigma>') \<leftarrow> reg_govt_shares attrs enc_attrs;
+      b' \<leftarrow> \<A>2 \<sigma> S;
+      return_spmf (b' = b)} ELSE coin_spmf"
+      using assms[unfolded no_sens_attr_def] 
+      by simp
+    also have "... = TRY do {
+      ((user0, user1), \<sigma>) \<leftarrow> \<A>1;
+      _ :: unit \<leftarrow> assert_spmf (valid_user user0 \<and> valid_user user1);
+      b :: bool \<leftarrow> coin_spmf;
+      let (attrs, sens_attrs) = users_attr_creation (if b then user0 else user1);
+      enc_attrs \<leftarrow> reg_enc_sens_attrs {};
+      (S, \<sigma>') \<leftarrow> reg_govt_shares attrs enc_attrs;
+      b' \<leftarrow> \<A>2 \<sigma> S;
+      return_spmf (b' = b)} ELSE coin_spmf"
+
+    also have "... = TRY do {
+      ((user0, user1), \<sigma>) \<leftarrow> \<A>1;
+      _ :: unit \<leftarrow> assert_spmf (valid_user user0 \<and> valid_user user1);
+      b :: bool \<leftarrow> coin_spmf;
+      enc_attrs_b \<leftarrow> reg_enc_sens_attrs {};
+      b' :: bool \<leftarrow> \<A>2 \<sigma> enc_attrs_b;
+      return_spmf (b' = b)} ELSE coin_spmf"
+      using assms[unfolded no_sens_attr_def] 
+      by simp
+    also have "... = TRY do {
+      ((user0, user1), \<sigma>) \<leftarrow> \<A>1;
+      _ :: unit \<leftarrow> assert_spmf (valid_user user0 \<and> valid_user user1);
+      enc_attrs_b \<leftarrow> reg_enc_sens_attrs {};
+      b' :: bool \<leftarrow> \<A>2 \<sigma> enc_attrs_b;
+      map_spmf((=) b') coin_spmf} ELSE coin_spmf"
+      by(simp add: map_spmf_conv_bind_spmf)
+    also have "... = coin_spmf" 
+      by(auto simp add: bind_spmf_const map_eq_const_coin_spmf try_bind_spmf_lossless2' scale_bind_spmf weight_spmf_le_1 scale_scale_spmf)
+    ultimately show ?thesis  
+      by(simp add: spmf_of_set)
+  qed
+  thus ?thesis 
+    by(simp add: perfect_sens_attrs_hiding_def sens_attrs_hiding_advantage_def)
+qed
+
+
+end *)
