ID_system_formalisation/Germany.thy
@@ -1,0 +1,27 @@
+theory Germany imports
+  Decentralised_Model
+begin
+
+locale germany =
+  fixes gen_card :: "'user \<Rightarrow> ('card \<times> 'chip) spmf"
+    and auth :: "('card \<times> 'chip) \<Rightarrow> ('user, 'query_out) query \<Rightarrow> 'query_out spmf"
+    and valid_user :: "'user \<Rightarrow> bool"
+    and valid_query :: "('user, 'query_out) query \<Rightarrow> bool"
+  assumes lossless_gen_card: "lossless_spmf (gen_card user)"
+begin
+
+definition register :: "'user \<Rightarrow> (('card \<times> 'chip) \<times> (unit, unit) govt_store_data) spmf"
+  where 
+    "register user = do {
+      (card, chip) \<leftarrow> gen_card user;
+      return_spmf ((card, chip), ({}, {}))}"
+
+sublocale germany_id: decentralised_id register auth valid_user valid_query 
+  unfolding decentralised_id_def by(simp add: register_def lossless_gen_card)
+
+lemma "germany_id.perfect_sens_attrs_hiding \<A>"
+proof(rule germany_id.no_sens_attrs_imp_perfect_sens_attrs_hiding)
+  show " \<forall>user token store_non_sens_attr store_sens_attr. (token, store_non_sens_attr, store_sens_attr) \<in> set_spmf (register user) \<longrightarrow> store_sens_attr = {}"
+    by(simp add: register_def)
+qed
+
